Knot example complete

knot/KnotA.v
@@ -1,170 +1,124 @@
 Require Import CRIS.
-
 Require Import KnotHeader.
 Require Import APCHeader APC.
 
-Set Implicit Arguments.
+Local Definition RA := authUR (optionUR (exclR (optionO (natO -d> natO)))).
 
-Section RA.
-  Context `{!crisG Γ Σ α β τ _S _I}.
-
-  Local Definition RA :=
-    authUR (optionUR (exclR (optionO (natO -d> natO)))).
-
-  Class knotG `{!crisG Γ Σ α β τ _S _I} := {
-    knot_inG :: inG RA Γ;
-  }.
-  Definition knotΓ : HRA := #[RA].
-  Global Instance subG_knotG : subG knotΓ Γ → knotG.
-  Proof. solve_inG. Defined.
-End RA.
-Hint Unfold subG_knotG knot_inG : GRA_index.
-
-(* Initial Resource *)
-Definition knot_init_res : RA := (● (Excl' None) ⋅ ◯ (Excl' None)).
-
-Lemma knot_init_valid : ✓ knot_init_res.
-Proof. rewrite /knot_init_res auth_both_valid //. Qed.
-Definition ir_knotRA : DRA_mk RA := knot_init_res.
-Lemma ir_knotRA_valid : ✓ ir_knotRA.
-Proof. eapply knot_init_valid. Qed.
-
-Definition ir_knotAΓ : knotΓ := *[Some (ir_knotRA)].
+Class knotGpreS `{!crisG Γ Σ α β τ _S _I} := {
+  #[local] knot_inG :: inG RA Γ;
+}.
+Class knotGS `{!crisG Γ Σ α β τ _S _I} := {
+  #[local] knotG_knotGpreS :: knotGpreS;
+  knot_name : gname;
+}.
+Definition knotΓ : HRA := #[RA].
+Global Instance subG_knotG `{!crisG Γ Σ α β τ _S _I} : subG knotΓ Γ → knotGpreS.
+Proof. solve_inG. Qed.
 
 Module KnotA. Section KnotA.
-  Context `{!crisG Γ Σ α β τ _S _I}.
-  Context `{_memG: !memG}.
-  Context `{_knotG: !knotG}.
-
-  (* Resources *)
+  Context `{!crisG Γ Σ α β τ _S _I, !concGS, !memGS, !knotGS}.
 
   Global Instance leibniz_equiv_discrete_funO_natO_natO: LeibnizEquiv (natO -d> natO).
   Proof.
-    ii. assert ((x: nat → nat) = (y: nat → nat)).
-    { apply func_ext. intro z. specialize (H z). ss. } ss.
+    intros ?? EQ. assert ((x: nat → nat) = (y: nat → nat)).
+    { apply func_ext. intro z. specialize (EQ z). ss. } ss.
   Qed.
 
-  Definition knot_full (f: option (nat → nat)) : iProp Σ :=
-    own base_γ (● (Some (Excl (f: optionO (natO -d> natO))))).
+  Definition knot_full (f : option (nat → nat)) : iProp Σ :=
+    own knot_name (● (Some (Excl (f : optionO (natO -d> natO))))).
   Definition knot_frag (f: option (nat → nat)) : iProp Σ := 
-    own base_γ (◯ (Some (Excl (f: optionO (natO -d> natO))))).
+    own knot_name (◯ (Some (Excl (f : optionO (natO -d> natO))))).
 
-  Definition knot_init: iProp Σ := knot_frag None.
-
-  Lemma knot_ra_merge
-      (f0 f1: optionO (natO -d> natO))
-    :
-    (knot_full f0) -∗ (knot_frag f1) -∗ (⌜f1 ≡ f0⌝).
+  Lemma knot_ra_merge (f0 f1 : optionO (natO -d> natO)) :
+    knot_full f0 -∗ knot_frag f1 -∗ ⌜f1 = f0⌝.
   Proof.
     iIntros "H0 H1". iCombine "H0 H1" as "H" gives %WF.
     iPureIntro. rewrite auth_both_valid_discrete in WF. des.
-    apply Excl_included in WF. et.
+    apply Excl_included in WF. inv WF; eauto.
   Qed.
 
-  Lemma knot_frag_unique
-      (f0 f1: optionO (natO -d> natO))
-    :
-      (knot_frag f0) -∗ (knot_frag f1) -∗ (⌜False⌝).
+  Lemma knot_frag_unique (f0 f1 : optionO (natO -d> natO)) :
+    knot_frag f0 -∗ knot_frag f1 -∗ ⌜False⌝.
   Proof.
     iIntros "H0 H1". iCombine "H0 H1" as "H" gives %WF. exfalso.
-    rewrite -auth_frag_op auth_frag_valid in WF. inv WF.
+    rewrite -auth_frag_op auth_frag_valid // in WF.
   Qed.
 
-  Lemma knot_full_unique
-      (f0 f1: optionO (natO -d> natO))
-    :
-      (knot_full f0) -∗ (knot_full f1) -∗ (⌜False⌝).
+  Lemma knot_full_unique (f0 f1 : optionO (natO -d> natO)) :
+    knot_full f0 -∗ knot_full f1 -∗ ⌜False⌝.
+  Proof. iIntros "H0 H1". iCombine "H0 H1" as "H" gives %[]; ss. Qed.
+
+  Lemma knot_update (f1 f2 : option (nat → nat)) :
+    knot_full f1 ∗ knot_frag f1 ==∗ knot_full f2 ∗ knot_frag f2.
   Proof.
-    iIntros "H0 H1". iCombine "H0 H1" as "H" gives %WF. exfalso.
-    inv WF; ss.
+    rewrite /knot_full /knot_frag -?own_op own_update; [iIntros "$"|].
+    by apply auth_update, option_local_update, exclusive_local_update.
   Qed.
 
-  Lemma auth_excl_both_update N
-      (old new: optionO (natO -d> natO))
-    :
-      own N (● Excl' old ⋅ ◯ Excl' old) ⊢ |==> own N (● Excl' new ⋅ ◯ Excl' new).
-  Proof.
-    apply own_update. apply auth_update. rewrite local_update_discrete. i.
-    split; ss. destruct mz; ss. destruct c; ss. inv H0.
-  Qed.
+  Variable (genv : GEnv.t) (sp_rec sp_fun : specmap).
 
-  (* Specifications *)
-
-Section KnotAS.
-
-  Variable genv: GEnv.t.
-  Variable SpRec: spl_type.
-  Variable SpFun: spl_type.
-  Variable SpPure: spl_type.
-
-  Definition var_points_to (var: string) (v: val): iProp Σ :=
+  Definition var_points_to (var : string) (v : val): iProp Σ :=
     match ((CEnv.load_genv genv).(CEnv.id2blk) var) with
-    | Some blk => mem_points_to_singleton (blk, 0%Z) 1%Qp v
+    | Some blk => (blk, 0%Z) ↦ v
     | None => True
     end.
 
-  Definition mrec_spec (f: nat -> nat) (INV: iProp Σ): fspec :=
+  Definition mrec_spec (f: nat → nat) (INV: iProp Σ): fspec :=
     fspec_apc (λ n: nat, 2 * n + 1)%ord
-      (fun (n: nat) =>
-          ((fun arg => (⌜arg = [Vint (Z.of_nat n)]↑ /\ (intrange_64 n)⌝ ∗ INV)%I),
-            (fun ret => (⌜ret = (Vint (Z.of_nat (f n)))↑⌝ ∗ INV)%I))).
+      (λ (n: nat),
+          ((λ arg, (⌜arg = [Vint (Z.of_nat n)]↑ /\ (intrange_64 n)⌝ ∗ INV)%I),
+            (λ ret, (⌜ret = (Vint (Z.of_nat (f n)))↑⌝ ∗ INV)%I))).
   
   Definition rec_spec: fspec :=
     fspec_apc (λ '(f, n), (2 * (n: nat) + 1)%ord)
-      (fun '(f, n) => 
-        ((fun varg => (⌜varg = [Vint (Z.of_nat n)]↑ /\ (intrange_64 n)⌝ ∗ knot_frag (Some f))%I),
-          (fun vret => (⌜vret = (Vint (Z.of_nat (f n)))↑⌝ ∗ knot_frag (Some f))%I))).
+      (λ '(f, n), 
+        ((λ varg, (⌜varg = [Vint (Z.of_nat n)]↑ /\ (intrange_64 n)⌝ ∗ knot_frag (Some f))%I),
+          (λ vret, (⌜vret = (Vint (Z.of_nat (f n)))↑⌝ ∗ knot_frag (Some f))%I))).
   
-  Definition fun_gen (f: nat -> nat): fspec :=
-    fspec_apc (λ n: nat, (2 * n)%ord)
-      (fun n => 
-        ((fun varg => (⌜∃ fb, varg = [Vptr (fb, 0%Z); Vint (Z.of_nat n)]↑ ∧ (intrange_64 n) ∧
-                        fb_has_spec_in genv SpRec fb rec_spec⌝
+  Definition fun_gen (f : nat → nat) : fspec :=
+    fspec_apc (λ n : nat, (2 * n)%ord)
+      (λ n, 
+        ((λ varg, (⌜∃ fb, varg = [Vptr (fb, 0%Z); Vint (Z.of_nat n)]↑ ∧ (intrange_64 n) ∧
+                        fb_has_spec_in genv sp_rec fb rec_spec⌝
                         ∗ knot_frag (Some f))%I),
-          (fun vret => (⌜vret = (Vint (Z.of_nat (f n)))↑⌝ ∗ knot_frag (Some f))%I))).
+          (λ vret, (⌜vret = (Vint (Z.of_nat (f n)))↑⌝ ∗ knot_frag (Some f))%I))).
 
-  Definition KnotRecSp: spl_type :=
-    Seal.sealing CRIS [(Some KnotHdr.rec, fsp_some rec_spec)].
+  Definition knot_rec_sp : specmap := {[speckey_fn KnotHdr.rec := fspec_to_rel rec_spec]}.
 
   Definition knot_spec : fspec :=
-    fspec_simple (X:=(nat -> nat))
-      (fun f => 
-        ((fun varg => (⌜∃ fb, varg = [Vptr (fb, 0%Z)]↑ ∧ 
-                        fb_has_spec_in genv SpFun fb (fun_gen f)⌝
-                        ∗ (∃ old, knot_frag old))%I,
-          (fun vret => (⌜∃ fb, vret = (Vptr (fb, 0%Z))↑ ∧
-                        fb_has_spec_in genv SpRec fb rec_spec⌝
-                        ∗ knot_frag (Some f))%I)))).
+    fspec_simple (X:=nat → nat)
+      (λ f, 
+        ((λ varg, (⌜∃ fb, varg = [Vptr (fb, 0%Z)]↑ ∧ fb_has_spec_in genv sp_fun fb (fun_gen f)⌝ ∗
+          (∃ old, knot_frag old))%I,
+        (λ vret, (⌜∃ fb, vret = (Vptr (fb, 0%Z))↑ ∧ fb_has_spec_in genv sp_rec fb rec_spec⌝ ∗
+          knot_frag (Some f))%I)))).
 
-  Definition KnotSp : spl_type :=
-    Seal.sealing CRIS 
-      [(Some KnotHdr.rec, fsp_some rec_spec);
-      (Some KnotHdr.knot, fsp_some knot_spec)].
-
-End KnotAS.
-
-Section KnotA.
-  (* Define Module *)
+  Definition knot_sp : specmap :=
+    {[speckey_fn KnotHdr.rec := fspec_to_rel rec_spec;
+      speckey_fn KnotHdr.knot := fspec_to_rel knot_spec]}.
 
   Definition scopes := ["Knot"].
 
-  Definition fnsems genv SpRec SpFun : fnsems_type :=
-    [(Some KnotHdr.rec, (true, wmask_all, scopes, (fsp_some rec_spec, pure_body)));
-     (Some KnotHdr.knot, (true, wmask_all, scopes, (fsp_some (knot_spec genv SpRec SpFun), fbody_trivial)))].
+  Definition fnsems : fnsemmap :=
+    {[Some KnotHdr.rec := Some (msk_scp scopes msk_true, (fsp_some rec_spec, pure_body));
+      Some KnotHdr.knot := Some (msk_scp scopes msk_true, (fsp_some (knot_spec), fbody_trivial))]}.
 
-  Program Definition smod genv SpRec SpFun : SMod.t :=
-  {|
+  Program Definition smod : SMod.t := {|
     SMod.scopes := scopes;
-    SMod.fnsems := fnsems genv SpRec SpFun;
-    SMod.initial_st := [];
+    SMod.fnsems := fnsems;
+    SMod.initial_st := ∅;
   |}.
-  Solve All Obligations with prove_scope.
-  Next Obligation. prove_nodup. Qed.
+  Solve All Obligations with mod_tac.
 
-  Definition init_cond genv : iProp Σ :=
-    ((var_points_to genv KnotHdr._f (Vint 0)) ∗ knot_full None)%I.
+  Definition init_cond : iProp Σ := (var_points_to KnotHdr._f (Vint 0) ∗ knot_full None)%I.
 
-  Definition t genv SpRec SpFun Sp :=
-    Seal.sealing CRIS (SMod.to_mod Sp (smod genv SpRec SpFun)).
-End KnotA.
+  Definition t sp := SMod.to_mod sp smod.
 End KnotA. End KnotA.
+
+Lemma knot_alloc `{!crisG Γ Σ α β τ _S _I, !knotGpreS} :
+  ⊢ o=> ∃ (_ : knotGS), KnotA.knot_full None ∗ KnotA.knot_frag None.
+Proof.
+  iMod (own_alloc (● (Excl' None) ⋅ ◯ (Excl' None))) as "[%γ [? ?]]".
+  { apply auth_both_valid_discrete; split; done. }
+  by iExists (Build_knotGS _ _ _ _ _ _ _ _ _ γ); iFrame.
+Qed.
