knot/KnotIAproof.v
@@ -1,56 +1,49 @@
 Require Import CRIS.
-Require Import KnotHeader KnotI KnotA MemHeader APCHeader APC APCA APCTactics Tactics.
-
-Set Implicit Arguments.
-
-Local Open Scope nat_scope.
+Require Import MemTactics.
+Require Import APCHeader APC APCA APCTactics Tactics.
+Require Import KnotI KnotA.
 
 Module KnotIA. Section KnotIA.
   Import KnotA APC APCA.
-  Context `{!crisG Γ Σ α β τ _S _I}.
-  Context `{_memG: !memG}.
-  Context `{_knotG: !knotG}.
-                 
+  Context `{!crisG Γ Σ α β τ _S _I, !concGS, !memGS, !knotGS}.
+
   (* 1. global environment *)
   Context (genv: GEnv.t).
-  (* 3. spec tables *)
-  Context (Sp : sp_type).
-  Context (SpRec SpFun SpMem SpPure: spl_type).
-  (* 4. hypotheses for genv *)
-  Context (GEnvWF: GEnv.wf genv).
-  Context (GEnvIncl: incl KnotGEnv.t genv).
-  (* 5. hypotheses for sp *)
-  Context (RecInSp: spl_sub KnotRecSp SpRec).
-  Context (APCInSp: sp_incl APCA.Sp Sp).
-  (* 6. hypotheses for pure sp *)
-  Context (FunInPure: spl_sub SpFun SpPure).
-  Context (PureInSp : sp_incl SpPure Sp).
 
-  Definition inv : iProp Σ :=
-    (∃ (f': optionO (natO -d> natO)) (fb': val),
+  (* 2. spec maps *)
+  Context (sp sp_rec sp_fun sp_mem sp_pure : specmap).
+
+  (* 3. hypotheses for genv *)
+  Context (GEnvWF : GEnv.wf genv).
+  Context (GEnvIncl : incl KnotGEnv.t genv).
+
+  (* 4. hypotheses for sp *)
+  Context (RecInSp: knot_rec_sp ⊆ sp_rec).
+  Context (APCInSp: APCA.sp ⊆ sp).
+
+  (* 5. hypotheses for pure sp *)
+  Context (FunInPure: sp_fun ⊆ sp_pure).
+  Context (PureInSp : sp_pure ⊆ sp).
+
+  Definition Ist : ist_type Σ := λ _ _,
+    (∃ (f' : optionO (natO -d> natO)) (fb' : val),
         (⌜∀ f (EQ: f' ≡ (Some f: optionO (natO -d> natO))),
             ∃ fb,
               (<<BLK: fb' = Vptr (fb, 0%Z)>>) /\
-              (<<FN: fb_has_spec_in genv SpFun fb (fun_gen genv SpRec f)>>)⌝)
+              (<<FN: fb_has_spec_in genv sp_fun fb (fun_gen genv sp_rec f)>>)⌝)
           ∗ (knot_full f')
           ∗ (var_points_to genv KnotHdr._f fb'))%I.
 
-  Definition Ist: alist key Any.t -> alist key Any.t -> iProp Σ :=
-    λ _ _, inv.
+  Local Notation APCA := (APCA.t sp_pure sp).
+  Local Notation MemA := (MemA.t sp_mem).
+  Local Notation KnotA := (KnotA.t genv sp_rec sp_fun sp).
+  Local Notation KnotAMod := (KnotA ★ MemA ★ APCA).
+  Local Notation KnotIMod := ((KnotI.t genv) ★ MemA ★ APCA).
+  Local Notation IstFull := (IstProd (IstSB KnotA.(Mod.scopes) Ist) IstEq).
 
-  Local Definition APCA := (APCA.t SpPure Sp).
-  Local Definition MemA := MemA.t.
-  Local Definition KnotA := (KnotA.t genv SpRec SpFun Sp).
-  Local Definition KnotAMod := (KnotA ★ MemA ★ APCA).
-  Local Definition KnotIMod := ((KnotI.t genv) ★ MemA ★ APCA).
-  Local Definition IstFull := (IstProd (IstSB KnotA.(Mod.scopes) Ist) IstEq).
-  
-  (*************)
-
-  Lemma simF_rec:
-    ISim.sim_fun open KnotAMod KnotIMod (KnotA.init_cond genv) IstFull (Some KnotHdr.rec).
+  Lemma simF_rec : ISim.sim_fun open KnotAMod KnotIMod IstFull (Some KnotHdr.rec).
   Proof using GEnvWF GEnvIncl RecInSp APCInSp FunInPure PureInSp.
-    init_simF.
+    iStartSim.
 
     (* SKINCL - SkEnv id2blk *)
     pose proof (@CEnv.incl_incl_env KnotGEnv.t genv) as INCLENV.
@@ -59,74 +52,71 @@ Module KnotIA. Section KnotIA.
     eapply INCLENV in GEnvIncl; et. unfold CEnv.incl_env in GEnvIncl.
     specialize (@GEnvIncl KnotHdr._f (Gvar 0%Z)↑) as SF.
     specialize (@GEnvIncl KnotHdr.rec Gfun↑) as SR.
-    hexploit SF; [right; right; left; ss|intro SKINCL_F].
-    hexploit SR; [right; left; ss|intro SKINCL_REC]. des. clear SF SR INCLENV.
+    hexploit SF; [right; right; left; ss|intros [blk_sf SKINCL_F]].
+    hexploit SR; [right; left; ss|intros [blk_sr SKINCL_REC]]. clear SF SR INCLENV.
 
     (* SKWF - SkEnv blk2id *)
     apply CEnv.load_genv_wf in GEnvWF. unfold CEnv.wf in GEnvWF.
-    specialize (GEnvWF KnotHdr.rec blk). apply GEnvWF in FIND; et. apply GEnvWF in FIND as FINDR.
+    (* specialize (GEnvWF KnotHdr.rec blk_sr). *)
+    apply GEnvWF in SKINCL_REC; et. apply GEnvWF in SKINCL_F as FINDR.
 
     (* Simulation Start *)
     (* SRC: precondition *)
-    steps_l. iDestruct "ASM" as "((%Y & FG) & %Q)"; des; subst; hss. steps_r.
+    steps_l. destruct _q as [f o]. iDestruct "ASM" as "(((-> & %) & FG) & %Q)". steps_r.
     iDestruct "IST" as (? ? ? ?) "(%ST & [% IST] & %E)"; des; subst.
-    iDestruct "IST" as (? ?) "(% & FL & VF)".
+    iDestruct "IST" as (? ?) "(%HIN & FL & VF)".
 
     (* RA: Set _f as a funciton pointer whose spec is "_f_spec" *)
-    iPoseProof (knot_ra_merge with "FL FG") as "%".
-    symmetry in H2. specialize (H1 _q1 H2). des; subst.
-    rename _q1 into _f_spec.
+    iPoseProof (knot_ra_merge with "FL FG") as "<-".
     
     (* TGT: get a block of _f *)
-    rewrite FIND0. hss. steps_r.
+    rewrite SKINCL_F. steps_r.
 
     (* TGT: load the function at the block of _f by inlining "load" *)
-    inline_r. rewrite /MemSpec.load.
-    steps_r. force_r (blk0, 0%Z, 1%Qp, (Vptr (fb, 0%Z))). forces_r.
-    iSplitL "VF".
-    { iSplit; eauto. unfold var_points_to. rewrite FIND0. iFrame. et. }
-    steps_r. iDestruct "GRT" as "[% [PT %]]"; subst. hss.
+    iEval (rewrite /var_points_to SKINCL_F) in "VF". load_r "VF".
+    hexploit (HIN f); eauto; intros [fb [EQ [? FBLOCK]]]; rewrite EQ /=.
 
     (* TGT: get blocks of the function pointer and "rec" *)
-    steps_r. dup FN. inv FN. rewrite FBLOCK. hss.
-    steps_r. rewrite FINDR; hss. steps_r.
+    steps_r. rewrite FBLOCK.
+    eapply GEnvWF in SKINCL_REC; rewrite SKINCL_REC. steps_r.
 
     (* SRC: unfold APC *)
-    steps_l. forces_l. iSplitR; et. steps_l.
-    inline_l. steps_l. iDestruct "ASM" as "%"; subst; hss.
+    rewrite /pure_body.
+    steps_l. simpl_sp. force_l. forces_l. iSplit; eauto. steps_l.
+    inline_l. steps_l. iDestruct "ASM" as "[-> <-]".
     steps_l. unfold apc_body, APC. force_l 1. steps_l. 
 
     (* call apc with fn *)
-    dup SPEC. inv SPEC.
-    apc_call_weaker "FL FG PT"; eauto.
+    pose proof SPEC as SPEC1. inv SPEC1.
+    iApply wsim_apc_src_call_tgt_weaker; [ | | |simpl_sp| | |iSplitL "FL FG VF"]; eauto.
     { instantiate (1 := 0). apply OrdArith.lt_from_nat. nia. }
-    { instantiate (1:= (2 * _q2)). eapply Ord.lt_le_lt; et. rewrite -OrdArith.mult_from_nat -OrdArith.add_from_nat. apply OrdArith.lt_from_nat. nia. }
-    { iSplitR "FL PT".
-      - unfold precond. ss. iFrame. iSplit.
-        + iPureIntro. eexists; esplits; et. econs; et.
-          econs; [|replace (fspec_to_rel rec_spec) with (fspec_flat (fsp_some rec_spec)) by ss; refl].
-          apply RecInSp. unfold KnotRecSp. unseal CRIS. ss.
-        + iPureIntro. eexists; esplits; et. rewrite -OrdArith.mult_from_nat. apply OrdArith.le_from_nat. nia. 
-      - iExists _, _, _, _. repeat (iSplit; et). iExists (Some _f_spec), _. iSplit.
-        + iPureIntro. i. esplits; et. instantiate (1:=fb). econs; et. inv EQ; et.
-        + unfold var_points_to. rewrite FIND0. iFrame.
+    { instantiate (1:= (2 * o)). eapply Ord.lt_le_lt; et.
+      rewrite -OrdArith.mult_from_nat -OrdArith.add_from_nat. apply OrdArith.lt_from_nat. nia.
     }
-    iDestruct "ISTPOST" as "[IST [% FG]]". hss.
-
-    (* TGT: steps tgt *)
-    steps_r. hss. steps_r.
+    { iSplitR "FL VF".
+      - ss. iFrame. iSplit.
+        + iPureIntro. eexists; esplits; et. econs; et.
+          { eapply GEnvWF; eauto. }
+          econs; [simpl_sp; eauto|].
+          iIntros (??) "%"; iExists _, _; iSplit; [done|iIntros "%% $ !> %%$//"].
+        + iPureIntro. eexists; esplits; et. rewrite -OrdArith.mult_from_nat. apply OrdArith.le_from_nat. nia. 
+      - iExists _, _, _, _. repeat (iSplit; et). iExists (Some f), _. iSplit.
+        + iPureIntro. intros ? temp; inv temp; esplits; et. econs; eauto.
+        + unfold var_points_to. rewrite SKINCL_F EQ. iFrame.
+    }
+    clear_st. iIntros (st_src st_tgt ret) "IST".
+    iDestruct "IST" as "[IST [-> FG]]". steps_r.
 
     (* SRC: change to skip *)
-    apc_l. steps_l. forces_l. iSplit; et. steps_l. forces_l. iSplitL "FG"; iFrame; et.
+    iApply wsim_apc_src. steps_l. forces_l. iSplit; et. steps_l. forces_l. iSplitL "FG"; iFrame; et.
 
     step. by iFrame.
-    Unshelve. all: ss.
+    Unshelve. all: try exact (tt↑).
   (*SLOW*)Qed.
 
-  Lemma simF_knot:
-    ISim.sim_fun open KnotAMod KnotIMod (KnotA.init_cond genv) IstFull (Some KnotHdr.knot).
+  Lemma simF_knot : ISim.sim_fun open KnotAMod KnotIMod IstFull (Some KnotHdr.knot).
   Proof using GEnvWF GEnvIncl RecInSp APCInSp FunInPure PureInSp.
-    init_simF.
+    iStartSim.
 
     (* SKINCL *)
     pose proof (@CEnv.incl_incl_env KnotGEnv.t genv) as INCLENV.
@@ -141,38 +131,33 @@ Module KnotIA. Section KnotIA.
     specialize (GEnvWF KnotHdr.rec blk). apply GEnvWF in FIND; et. apply GEnvWF in FIND as FINDR.
 
     (* SRC: precondition *)
-    steps_l.
-    rename _q into new_spec.
-    iDestruct "ASM" as "(%Q & (%FB & [%old OLD]))". des; subst. hss. steps_r.
+    steps_l. rename _q into new_spec.
+    iDestruct "ASM" as "(%Q & (%FB & [%old OLD]))". des; subst. steps_r.
     iDestruct "IST" as (? ? ? ?) "(%ST & [% IST] & %E)"; des; subst.
-    iDestruct "IST" as (? ?) "(% & FL & VF)".
+    iDestruct "IST" as (? ?) "(%HIN & FL & VF)".
 
     (* RA: unify the infomation of f_spec *)
-    iPoseProof (knot_ra_merge with "FL OLD") as "%". symmetry in H2.
-    assert (REFL: knot_full f' ⊢ knot_full old). { iIntros "F". rewrite /knot_full H2. ss. }
-    iPoseProof (REFL with "FL") as "FL".
-    rewrite FIND0; hss. steps_r.
+    iPoseProof (knot_ra_merge with "FL OLD") as "->".
+    (* iPoseProof (REFL with "FL") as "FL". *)
+    rewrite FIND0. steps_r.
     
     (* TGT: save a function by calling "store" *)
-    steps_r. inline_r. steps_r.
-    force_r (blk0, 0%Z, _, Vptr (fb, 0%Z)). forces_r. iSplitL "VF".
-    { iSplit; et. unfold var_points_to. rewrite FIND0; eauto. }
-    steps_r. iDestruct "GRT" as "[% [VF %]]". hss; steps_r.
+    rewrite /var_points_to FIND0. store_r "VF".
 
     (* RA: update spec *)
-    rewrite FINDR; hss. steps_r.
-    iCombine "FL OLD" as "SPEC".
-    iPoseProof (auth_excl_both_update with "SPEC") as ">[FL FG]".
+    rewrite FINDR. steps_r.
+    iMod (knot_update _ (Some new_spec) with "[FL OLD]") as "[FL FG]"; first iFrame.
+    (* iCombine "FL OLD" as "SPEC". *)
+    (* iPoseProof (auth_excl_both_update with "SPEC") as ">[FL FG]". *)
 
     (* finish reasoning *)
-    steps_l. force_l. steps_l. force_l. force_l.
-    iSplitL "FG"; iFrame; et.
-    { iSplit; et. iPureIntro. eexists. esplit; et. econs; et.
-      econs; [|replace (fspec_to_rel rec_spec) with (fspec_flat (fsp_some rec_spec)) by ss; refl].
-      apply RecInSp. unfold KnotRecSp. unseal CRIS. ss.
+    force_l. steps_l. force_l. force_l.
+    iSplitL "FG".
+    { iSplitR; et. iSplitR; eauto. iPureIntro. eexists. esplit; et. econs; et.
+      econs; [simpl_sp; ss|].
+      iIntros (??) "%"; iExists _, _; iSplit; [done|iIntros "%% $ !> %%$//"].
     }
-    steps_l.
-    hss. steps_r. step. iSplit; et.
+    step. iSplit; et.
 
     (* check IST *)
     inv FB0. des.
@@ -182,21 +167,19 @@ Module KnotIA. Section KnotIA.
     { unfold var_points_to. des_ifs. }
   Qed.
 
-  Theorem sim : ISim.t open KnotAMod KnotIMod (KnotA.init_cond genv) IstFull.
+  Lemma sim : ISim.t open KnotAMod KnotIMod (KnotA.init_cond genv) IstFull.
   Proof.
     init_sim.
-    - split; eauto. iIntros "[VF FL]". iModIntro. iSplit; et.
-      { iPureIntro. split; ss. }
-      { unfold Ist, inv. iExists None, _. iSplit; iFrame; et. iPureIntro. ii. inv EQ. }
-    - apply simF_rec; et.
-    - apply simF_knot; et.
+    { apply simF_rec. }
+    { apply simF_knot. }
+    { iIntros "[VF FL]". iExists _, _, _, _. iSplit; et. iSplit; eauto.
+      iSplit; iFrame; et. iPureIntro. ii. inv EQ.
+    }
   Qed.
 
-  Theorem ctxr :
+  Lemma ctxr :
     ctx_refines
-      (KnotA.t genv SpRec SpFun Sp ★ MemA ★ APCA.t SpPure Sp,
-        KnotA.init_cond genv)
-      (KnotI.t genv ★ MemA ★ APCA.t SpPure Sp,
-        emp%I).
+      (KnotA.t genv sp_rec sp_fun sp ★ MemA ★ APCA.t sp_pure sp, KnotA.init_cond genv)
+      (KnotI.t genv ★ MemA ★ APCA.t sp_pure sp,                  emp%I).
   Proof. eapply main_adequacy, sim; eauto. Qed.
 End KnotIA. End KnotIA.
