knot/KnotMainIAproof.v
@@ -1,108 +1,112 @@
 Require Import CRIS.
-
-Require Import KnotHeader KnotMainHeader KnotMainI KnotMainA KnotA KnotI KnotIAproof.
-Require Import APCHeader APC APCA APCC APCTactics.
-
-Set Implicit Arguments.
+Require Import KnotMainI KnotMainA KnotA.
+Require Import APCTactics APC APCC APCHeader.
 
 Module KnotMainIA. Section KnotMainIA.
   Import KnotA KnotMainA APCA.
-  Context `{CrisG: !crisG Γ Σ α β τ _S _I}.
-  Context `{MemG: !memG}.
-  Context `{KnotG: !knotG}.
+  Context `{!crisG Γ Σ α β τ _S _I, !concGS, !memGS, !knotGS}.
 
   (* 1. global environment *)
   Context (genv: GEnv.t).
-  (* 3. spec tables *)
-  Context (Sp: sp_type).
-  Context (SpRec SpFun SpPure: spl_type).
-  (* 4. hypotheses for genv *)
-  Context (GEnvWF: GEnv.wf genv).
-  Context (GEnvIncl: incl KnotMainGEnv.t genv).
-  (* 5. hypotheses for sp *)
-  Context (MainInFun: spl_sub (MainFunSp genv SpRec) SpFun).
-  Context (KnotInSp: sp_incl KnotRecSp Sp).
-  Context (APCInSp: sp_incl APCA.Sp Sp).
-  (* 6. hypotheses for pure sp *)
-  Context (RecInSpPure: spl_sub SpRec SpPure).
-  Context (PureInGlobal : sp_incl SpPure Sp).
+  (* 2. spec tables *)
+  Context (sp sp_rec sp_fun sp_pure sp_mem : specmap).
+  (* 3. hypotheses for genv *)
+  Context (GEnvWF : GEnv.wf genv).
+  Context (GEnvIncl : incl KnotMainGEnv.t genv).
+  (* 4. hypotheses for sp *)
+  Context (MainInFun : (main_fun_sp genv sp_rec) ⊆ sp_fun).
+  Context (KnotInSp : knot_rec_sp ⊆ sp).
+  Context (APCInSp : APCA.sp ⊆ sp).
+  (* 5. hypotheses for pure sp *)
+  Context (RecInSpPure : sp_rec ⊆ sp_pure).
+  Context (PureInGlobal : sp_pure ⊆ sp).
 
-  Local Definition APCA := (APCA.t SpPure Sp).
-  Local Definition MemA := MemA.t.
-  Local Definition KnotA := (KnotA.t genv SpRec SpFun Sp).
-  Local Definition KnotAMod := (KnotA ★ MemA ★ APCA).
-  Local Definition KnotMainA := (KnotMainA.t true genv SpRec Sp).
-  Local Definition KnotMainI := (KnotMainI.t genv).
-  Local Definition KnotMainAMod := (KnotMainA ★ KnotAMod).
-  Local Definition KnotMainIMod := (KnotMainI ★ KnotAMod).
-  Local Definition IstFull := (IstProd (IstSB KnotMainA.(Mod.scopes) IstTrue) IstEq).
-  
-  (*************)
+  Local Notation APCA := (APCA.t sp_pure sp).
+  Local Notation MemA := (MemA.t sp_mem).
+  Local Notation KnotA := (KnotA.t genv sp_rec sp_fun sp).
+  Local Notation KnotAMod := (KnotA ★ MemA ★ APCA).
+  Local Notation KnotMainA := (KnotMainA.t genv sp_rec true sp).
+  Local Notation KnotMainI := (KnotMainI.t genv).
+  Local Notation KnotMainAMod := (KnotMainA ★ KnotAMod).
+  Local Notation KnotMainIMod := (KnotMainI ★ KnotAMod).
+  Local Notation IstFull := (IstProd (IstSB KnotMainA.(Mod.scopes) IstTrue) IstEq).
 
-  Lemma simF_fib:
-    ISim.sim_fun open KnotMainAMod KnotMainIMod KnotMainA.init_cond IstFull (Some KnotMainHdr.fib).
+  Lemma simF_fib : ISim.sim_fun open KnotMainAMod KnotMainIMod IstFull (Some KnotMainHdr.fib).
   Proof using APCInSp GEnvIncl GEnvWF KnotInSp MainInFun PureInGlobal RecInSpPure.
-    init_simF.
+    iStartSim.
 
-    steps_l. iDestruct "ASM" as "[[% INV] %]". des; subst. hss.
-    steps_r. inv H3. des. rewrite FBLOCK; hss. steps_r.
-    unfold assume. assert (T:true) by auto. force_r T. steps_r.
+    steps_l. destruct _q as [n I]; s. iDestruct "ASM" as "[[[%fb [-> [% %Hspec]]] I] [%vo [-> %]]]".
+    steps_r. inv Hspec. rewrite FBLOCK. steps_r.
+    unfold assume. unshelve force_r; eauto. steps_r.
     des_ifs.
     { (* base case *)
-      steps_r. steps_l. forces_l. iSplitR; et. steps_l.
+      rewrite /APC.pure_body. steps_l. simpl_sp. forces_l. iSplitR; et. steps_l.
       inline_l. steps_l.
-      iDestruct "ASM" as "%"; des; subst; hss. steps_l.
-      unfold apc_body, APC. force_l 0. steps_l. 
+      iDestruct "ASM" as "[-> <-]". steps_l.
+      unfold APC. force_l 0. steps_l.
+
       (* SRC: change to skip *)
-      apc_l. steps_l. forces_l. iSplitR; et. steps_l.
-      forces_l. iSplitL "INV"; iFrame; et.
-      assert (_q1 >= 0)%Z by nia. assert (_q1 = 1 \/ _q1 = 0) by nia. assert (Z.of_nat (Fib _q1) = 1)%Z.
+      iApply wsim_apc_src. steps_l. forces_l. iSplitR; et. steps_l.
+      forces_l. iSplitL "I"; iFrame; et.
+      assert (n = 1 \/ n = 0) by nia. assert (Hn : Z.of_nat (Fib n) = 1%Z).
       { des; subst; reflexivity. }
-      rewrite H3. step. iSplit; et.
+      rewrite Hn. step. iSplit; et.
     }
     { (* recursive call *)
-      steps_r. steps_l. forces_l. iSplitR; et. steps_l.
+      steps_r. rewrite /pure_body. steps_l. simpl_sp. forces_l. iSplitR; et. steps_l.
       inline_l. steps_l.
-      iDestruct "ASM" as "%"; des; subst; hss. steps_l. unfold apc_body, APC.
+      iDestruct "ASM" as "[-> <-]". steps_l. unfold APC.
       force_l 2. steps_l.
-      
+
       (* first call - rec(n - 1) *)
       dup SPEC. inv SPEC.
-      apc_call_weaker "IST INV"; et.
+      apc_call_weaker ""; et.
       { instantiate (1 := 1). apply OrdArith.lt_from_nat. ss. }
-      { instantiate (1 := (2 * (_q1 - 1) + 1)%ord). eapply Ord.lt_le_lt; [|et]. rewrite -!OrdArith.mult_from_nat -OrdArith.add_from_nat. apply OrdArith.lt_from_nat. nia. }
-      { unfold precond. ss. instantiate (1:= (_q1 - 1) ). iFrame. iSplit; et. iSplit; et.
-        - iPureIntro. repeat f_equal. nia.
-        - iPureIntro. unfold intrange_64 in *.
-          bsimpl; des; split; des_sumbool; repeat destruct Z_le_gt_dec; unfold min_64, max_64, modulus_64_half in *; try nia; ss.
+      { instantiate (1 := (2 * (n - 1) + 1)%ord). eapply Ord.lt_le_lt; [|et].
+        rewrite -!OrdArith.mult_from_nat -OrdArith.add_from_nat. apply OrdArith.lt_from_nat. nia. 
+      }
+      iSplitL "IST I".
+      { ss. instantiate (1:= (n - 1)). iFrame. iSplit; et.
+        - iPureIntro. split.
+          { repeat f_equal. lia. }
+          { unfold intrange_64 in *.
+            bsimpl; des; split; des_sumbool;
+            repeat destruct Z_le_gt_dec; unfold min_64, max_64, modulus_64_half in *; try nia; ss.
+          }
         - iPureIntro. eexists; esplits; et. refl. 
       }
-      iDestruct "ISTPOST" as "[IST [% INV]]". subst. steps_r. hss. steps_r.
+      clear_st. iIntros (st_src st_tgt ret) "[IST [-> I]]".
+      steps_r.
 
       (* second call - rec(n - 2) *)
-      apc_call_weaker "IST INV"; et.
+      apc_call_weaker ""; et.
       { instantiate (1:=0). apply OrdArith.lt_from_nat. ss. }
-      { instantiate (1 := (2 * (_q1 - 1))%ord). eapply Ord.lt_le_lt; [|et]. rewrite -!OrdArith.mult_from_nat. eapply OrdArith.lt_from_nat. nia. }
-      { iFrame. instantiate (1:= (_q1 - 2)). iSplit; et. iSplit; et.
-        - iPureIntro. repeat f_equal. nia.
-        - iPureIntro. unfold intrange_64 in *.
-          bsimpl; des; split; des_sumbool; repeat destruct Z_le_gt_dec; unfold min_64, max_64, modulus_64_half in *; try nia; ss.
-        - iPureIntro. eexists; esplits; et. rewrite -!OrdArith.mult_from_nat -OrdArith.add_from_nat. eapply OrdArith.le_from_nat. nia.
+      { instantiate (1 := (2 * (n - 1))%ord). eapply Ord.lt_le_lt; [|et].
+        rewrite -!OrdArith.mult_from_nat. eapply OrdArith.lt_from_nat. nia.
       }
-      iDestruct "ISTPOST" as "[IST [% INV]]". subst. steps_r. hss. steps_r.
+      { iFrame. instantiate (1:= (n - 2)). iSplit; et.
+        { iPureIntro. splits; first (repeat f_equal; nia).
+          { unfold intrange_64 in *.
+            bsimpl; des; split; des_sumbool; repeat destruct Z_le_gt_dec;
+              unfold min_64, max_64, modulus_64_half in *; try nia; ss.
+          }
+          eexists; esplits; et. rewrite -!OrdArith.mult_from_nat -OrdArith.add_from_nat.
+          eapply OrdArith.le_from_nat. nia.
+      }
+        clear_st. iIntros (st_src st_tgt ret) "[IST [-> I]]". steps_r.
 
-      apc_l. steps_l. forces_l. iSplit; et. steps_l. forces_l. iFrame. iSplit; et.
+        iApply wsim_apc_src. steps_l. forces_l. iSplit; et. steps_l. forces_l. iFrame. iSplit; et.
 
-      step. iSplit; et.
-      iPureIntro. repeat f_equal. rewrite unfold_fib; nia.
+        step. iSplit; et.
+        iPureIntro. repeat f_equal. rewrite unfold_fib; nia.
+      }
     }
-    Unshelve. all: ss. exact (0↑).
+    Unshelve. all: exact (0↑).
   (*SLOW*)Qed.
 
-  Lemma simF_main:
-    ISim.sim_fun open KnotMainAMod KnotMainIMod KnotMainA.init_cond IstFull None.
+  Lemma simF_main : ISim.sim_fun open KnotMainAMod KnotMainIMod IstFull None.
   Proof using APCInSp GEnvIncl GEnvWF KnotInSp MainInFun PureInGlobal RecInSpPure.
-    init_simF.
+    iStartSim.
 
     (* SKINCL *)
     pose proof (@CEnv.incl_incl_env KnotMainGEnv.t genv) as INCLENV.
@@ -110,124 +114,124 @@ Module KnotMainIA. Section KnotMainIA.
     eapply INCLENV in GEnvIncl; et. unfold CEnv.incl_env in GEnvIncl.
     specialize (@GEnvIncl KnotMainHdr.fib Gfun↑) as SF.
     hexploit SF; [left; ss|intro SKINCL_F].
-    des. clear SF INCLENV. inv KnotInSp.
+    des. clear SF INCLENV.
 
     (* SKWF *)
     apply CEnv.load_genv_wf in GEnvWF. unfold CEnv.wf in GEnvWF.
     specialize (GEnvWF KnotMainHdr.fib blk). apply GEnvWF in FIND; et. apply GEnvWF in FIND as FINDF.
 
     (* SRC: precondition *)
-    steps_l. destruct _q; ss. iDestruct "IST" as "[% FG]". des; subst. hss.
+    steps_l. iDestruct "ASM" as "[-> [-> FG]]". steps_l.
 
     (* TGT: find a block of the function "fib" using SKINCL *)
-    steps_r. rewrite FINDF; hss. steps_r.
+    steps_r. rewrite FINDF. steps_r.
 
     (* TGT: inlining "fib" *)
-    inline_r. steps_r. force_r Fib. forces_r. iSplitL "FG"; et.
+    inline_r. force_r Fib. forces_r. iSplitL "FG"; et.
     { (* prove the precondition of "fib" *)
       iFrame. iSplit; et. iPureIntro. eexists. esplits; et. econs; esplits; et.
-      eapply fn_has_weaker_spec_in.
-      { econs; [|instantiate (2:= Some (fspec_to_rel _)); s; refl].
-        apply MainInFun. unfold MainFunSp. unseal CRIS. ss. }
-      { unfold fspec_imply, precond, postcond, fun_gen, fib_spec, fun_gen, fib_spec, fspec_apc; ss. 
-        ii. rr in ValidSP; des; subst. eexists _, _; split; [rr;et|].
-        instantiate (1:= (x, (knot_frag (Some Fib))%I)). split; red.
-        { i. iIntros "[[% FG] %]". unfold precond, fun_gen, fib_spec; ss.
-          des; subst; hss. iModIntro. iSplit; et. iSplit; et; cycle 1.
-          iPureIntro. exists fb. esplits; et. inv H5. econs; et. eapply fn_has_weaker_spec_in; et.
-          unfold fspec_imply, precond, postcond, fun_gen, fib_spec, fun_gen, fib_spec, fspec_apc; ss.
-          ii. rr in ValidSP; des; subst. eexists _, _; split; [rr; et|]. split; red.
-          { red. instantiate (1:=(_, x0)). ss. iIntros; iFrame; et. }
-          { i. ss. iIntros; et. }
-        }
-        { i. ss. iIntros; et. }
-      }
+      econs.
+      { simpl_sp; ss. }
+      iIntros (P Q) "[% [-> ->]]"; iExists _, _; iSplit.
+      { iPureIntro; exists (x, knot_frag (Some Fib)); split; ss. }
+      iIntros (? ?) "[[% $] %] !>"; iSplit; eauto; iPureIntro; des; esplits; eauto.
+      inv H7. econs; eauto.
+      inv SPEC. econs; eauto.
+      iIntros (? ?) "[%n [-> ->]]". iPoseProof (WEAK with "[]") as "[% [% [% I]]]".
+      { iPureIntro. exists (Fib, n); split; ss. }
+      iExists _, _; iSplit; first eauto.
+      unfold_pre_post. iIntros (? ?) "[[% F] [% %]]"; iPoseProof ("I" with "[F]") as "?".
+      { iFrame. iSplit; eauto. }
+      eauto.
     }
 
     (* TGT: take a postcondition of "fib" *)
-    steps_r. iDestruct "GRT" as "[% [% FG]]"; des; subst; hss. steps_r. inv H3.
+    steps_r. iDestruct "GRT" as "[-> [[% [-> %]] FG]]". steps_r. inv H3.
 
     (* TGT: find a block of the function "rec" using the postcondition of "fib" *)
-    rewrite FBLOCK; hss. steps_r.
+    rewrite FBLOCK. steps_r.
     
     (* SRC: handle pure (APC) *)
     unfold pure. steps_l.
-    force_l 30%ord. steps_l. inv SPEC. force_l.
+    force_l 30%ord. steps_l. simpl_sp. force_l.
     forces_l. iSplitR; et. steps_l.
 
     (* SRC: inlining APC *)
-    inline_l. steps_l. iDestruct "ASM" as "%"; des; subst; hss. steps_l.
-    unfold apc_body, APC. force_l 1. steps_l. 
-    
+    inline_l. steps_l. iDestruct "ASM" as "%"; des; subst. steps_l.
+    unfold APC. force_l 1. steps_l. 
+    inv SPEC.
     (* SRC, TGT: call "fib" using APC tactic *)
     apc_call_weaker "FG"; et.
     { instantiate (1:=0). eapply OrdArith.lt_from_nat; et. }
-    { instantiate (1:= 29). eapply OrdArith.lt_from_nat; nia. }
-    { unfold precond. ss. instantiate (1:=(Fib, 10)). iFrame. iSplit; et.
-      { iPureIntro. eexists; esplits; ss.
-      rewrite -OrdArith.mult_from_nat -OrdArith.add_from_nat. apply OrdArith.le_from_nat; nia. }
-      { do 4 iExists []. ss. iPureIntro; hrepeat do 6 unfold_mod; ss; esplits; eauto; prove_scope. }
+    { instantiate (1:=29). hss. eapply OrdArith.lt_from_nat; nia. }
+    iSplitL "FG IST".
+    { ss. instantiate (1:=(Fib, 10)). iFrame. iSplit; et.
+      iPureIntro. eexists; esplits; ss.
+      rewrite -OrdArith.mult_from_nat -OrdArith.add_from_nat. apply OrdArith.le_from_nat; nia.
     }
-    iDestruct "ISTPOST" as "[IST [% FG]]". subst. steps_r. hss. steps_r.
+    clear_st. iIntros (st_src st_tgt ret) "[IST [-> FG]]". steps_r.
 
     (* SRC: jump APC *)
-    apc_l. steps_l. forces_l. iSplit; et. steps_l. 
+    iApply wsim_apc_src. steps_l. forces_l. iSplit; et. steps_l. force_l. steps_l.
+    force_l. iSplit; eauto. 
     step. iSplitR; et.
-    Unshelve. all: ss.
+    Unshelve. all: try exact (tt↑).
   (*SLOW*)Qed.
 
-  Theorem sim : ISim.t open KnotMainAMod KnotMainIMod KnotMainA.init_cond IstFull.
+  Lemma sim : ISim.t open KnotMainAMod KnotMainIMod emp%I IstFull.
   Proof.
     init_sim.
     (* - exfalso. revert H. unfold_mod; ss. *)
-    - eapply simF_fib; et.
-    - eapply simF_main; et.
+    { eapply simF_fib; et. }
+    { eapply simF_main; et. }
+    { iIntros "_"; repeat iExists _; iSplit; eauto. }
   Qed.
 
-  Theorem ctxr :
+  Lemma ctxr :
     ctx_refines
-      (KnotMainA.t true genv SpRec Sp
-        ★ KnotA.t genv SpRec SpFun Sp
-        ★ MemA.t
-        ★ APCA.t SpPure Sp,
-      KnotMainA.init_cond)
+      (KnotMainA.t genv sp_rec true sp
+        ★ KnotA.t genv sp_rec sp_fun sp
+        ★ MemA.t sp_mem
+        ★ APCA.t sp_pure sp,
+      emp%I)
       (KnotMainI.t genv
-        ★ KnotA.t genv SpRec SpFun Sp
-        ★ MemA.t
-        ★ APCA.t SpPure Sp,
+        ★ KnotA.t genv sp_rec sp_fun sp
+        ★ MemA.t sp_mem
+        ★ APCA.t sp_pure sp,
       emp%I).
   Proof. eapply main_adequacy, sim; eauto. Qed.
 
-  Theorem ctxr_close:
+  Lemma ctxr_close :
     ctx_refines
-      (KnotMainA.t false genv SpRec Sp ★ APCC.t Sp, emp%I)
-      (KnotMainA.t true  genv SpRec Sp ★ APCC.t Sp, emp%I).
-  Proof using CrisG MemG APCInSp GEnvIncl GEnvWF KnotInSp MainInFun PureInGlobal RecInSpPure.
+      (KnotMainA.t genv sp_rec false sp ★ APCC.t sp, emp%I)
+      (KnotMainA.t genv sp_rec true  sp ★ APCC.t sp, emp%I).
+  Proof using APCInSp GEnvIncl GEnvWF KnotInSp MainInFun PureInGlobal RecInSpPure.
     eapply main_adequacy.
     init_sim.
     (* { exfalso. revert H. hrepeat do 1 unfold_mod. i; inv H. } *)
-    { init_simF.
-      steps_l. iDestruct "ASM" as "[[% PRE] %]"; des; hss.
-      steps_l. force_l vo. steps_l. forces_l.
-      iSplitR; eauto. steps_l. force_r (_q1, _q2).
+    { iStartSim.
+      steps_l. case_match. iDestruct "ASM" as "[[% PRE] %]"; des; hss.
+      rewrite /pure_body. steps_l. simpl_sp. forces_l.
+      iSplitR; eauto. steps_l. force_r (n, u).
       forces_r. iSplitL "PRE".
       { iFrame; iPureIntro; esplits; eauto. }
-      hss. steps_r. iDestruct "GRT" as "%"; des; hss.
+      hss. steps_r. simpl_sp. steps_r. iDestruct "GRT" as "%"; des; hss.
       call "IST"; eauto.
+      iIntros (???) "IST".
       steps_l. steps_r. forces_r. iSplitL "ASM"; eauto.
       steps_r. iDestruct "GRT" as "[% POST]". forces_l.
       iSplitL "POST"; iFrame; eauto.
       step. iFrame; eauto.
     }
-    { init_simF.
-      steps_l. hss. iDestruct "IST" as "%"; des; hss.
-      steps_r. rewrite /pure. steps_r. inline_r. forces_r.
-      iDestruct "GRT" as "(% & %)". hss. iSplitR; et.
-      steps_r. forces_r. iSplitR; et.
-      steps_r. forces_l. step.
+    { iStartSim.
+      steps_l. hss. iDestruct "ASM" as "[% [% ?]]"; des; hss.
+      steps_l. forces_r. iFrame. iSplit; eauto. steps_r.
+      rewrite /pure. steps_r. simpl_sp. steps_r. inline_r. forces_r. iSplit; eauto. steps_r.
+      iDestruct "GRT" as "(% & %)". hss. forces_r. iSplitR; et.
+      steps_r. forces_l. iSplit; eauto. step.
       iSplit; eauto.
     }
-  Unshelve. all: et. exact IstTrue.
+    { instantiate (1:=const (const emp%I)). iIntros "_"; repeat iExists _; repeat iSplit; eauto. }
+  Unshelve. all: et. exact tt.
   (*SLOW*)Qed.
-
 End KnotMainIA. End KnotMainIA.
